LeanMqtt/Core/Codec.lean
@@ -3,14 +3,26 @@ import LeanMqtt.Core.Parser.Basic
 namespace Mqtt
 open Mqtt
 
+/-!
+# Codec
+
+This module containts type classes for _codecs_ which are types that can be
+serialized and parsed without an external context. For example, `String`s
+require the external context of a size to be parsed, while `Str`s don't.
+-/
+
 /--
   A typeclass for basic types that can be serialized and parsed without
-  any external information.
+  an external context.
 -/
 class Codec (α : Type) where
   parser : Parser α
   serialize : α → List UInt8
 
+/--
+  The main theorems we prove for the verified parser: _roundtrip_ and
+  _reconstruction_.
+-/
 class LawfulCodec (α : Type) [Codec α] where
   roundtrip : ∀ (a : α) {rest : List UInt8},
     Codec.parser.run (Codec.serialize a ++ rest) = some (a, rest)
