LeanMqtt/Packets/VarHeader/Proofs.lean
@@ -6,6 +6,7 @@ import LeanMqtt.Primitives.PredType.Proofs
 import LeanMqtt.Helpers.ParserTactics
 import LeanMqtt.Packets.VarHeader.Variations
 import LeanMqtt.Packets.VarHeader.Properties.Proofs
+import LeanMqtt.Packets.ReasonCode.Proofs
 
 namespace Mqtt
 open Mqtt
@@ -37,7 +38,7 @@ theorem Var_Connect.reconstruct
 theorem Var_Connack.roundtrip (v : Var_Connack) {rest : List UInt8} :
     Var_Connack.parser.run (v.serialize ++ rest) = some (v, rest) := by
   simp [Var_Connack.parser, Var_Connack.serialize]
-  simp [UInt8.roundtrip, Properties.roundtrip, PredType.roundtrip]
+  simp [ReasonCode.roundtrip, Properties.roundtrip, PredType.roundtrip]
 
 theorem Var_Connack.reconstruct {v : Var_Connack} {input rest : List UInt8} :
     Var_Connack.parser.run input = some (v, rest) → input = v.serialize ++ rest := by
@@ -49,7 +50,7 @@ theorem Var_Connack.reconstruct {v : Var_Connack} {input rest : List UInt8} :
   finish_parser h → h_v
   subst h_v
   rw [PredType.reconstruct ConnackFlagsProp h_ack_flagsVal,
-    UInt8.reconstruct h_rcodeVal,
+    ReasonCode.reconstruct h_rcodeVal,
     Properties.reconstruct h_propsVal]
   simp only [List.append_assoc]
 
